WIP

Clap/eDSLState/HashCons/EvalButActuallyGood.lean
@@ -22,13 +22,23 @@ def evalWithCache {p}
   if e < cache.size
   then cache
   else
-    match σ[e]? with
+    match σ[cache.size]? with
     | .none => cache
     | .some expr =>
       let val := evalCore varStore expr cache
       evalWithCache varStore e (cache.push val) σ
   termination_by (e + 1) - cache.size
   decreasing_by grind
+
+def state : HashConsSt 37 where
+  exprs := #[
+    .c 3,
+    .c 2,
+    .binary_op 0 1 .add
+  ]
+  wellFormed := by decide
+
+#eval evalWithCache {} 2 #[] state
 
 def eval {p} (varStore : VarStore p) (e : ExprRef) (σ : HashConsSt p) : Option (ZMod p) :=
   (evalWithCache varStore e #[] σ)[e]!
@@ -41,5 +51,57 @@ abbrev evalM {p} (varStore : VarStore p) (e : HashConsM p ExprRef) : HashConsM p
   return [varStore,state|expr]
 
 notation "[" varStore "," state "|" "←" x "]" => HashConsM.run (evalM varStore x) state
+
+section Prefix
+
+lemma Array.size_eq_zero_of_isPrefixOf_size_eq_zero
+  {T} [BEq T] [LawfulBEq T]
+  (a b: Array T)
+  (h_prefix : a.isPrefixOf b = true)
+  (h_size : b.size = 0)
+:
+  a.size = 0
+:= by
+  rewrite [←Array.isPrefixOf_toList] at h_prefix
+  grind
+
+lemma evalCache_of_lt_prefix
+  {p : ℕ}
+  {varStore : VarStore p}
+  {e : ExprRef}
+  {cache : ValueCache p}
+  {σ σ' : HashConsSt p}
+  (h_prefix : σ.exprs.isPrefixOf σ'.exprs)
+  (h_lt_prefix : e < σ.exprs.size)
+:
+  evalWithCache varStore e cache σ =
+  evalWithCache varStore e cache σ'
+:= by
+  induction h: e + 1 - cache.size generalizing cache with
+  | zero =>
+    unfold evalWithCache
+    grind
+  | succ n ih =>
+    unfold evalWithCache
+    split_ifs
+    . rfl
+    . have : cache.size < σ.exprs.size := by grind
+      have : σ[cache.size]? = σ'[cache.size]? := by
+        simp
+        rewrite [←Array.getElem?_toList, ←Array.getElem?_toList]
+        have : σ.exprs.toList.isPrefixOf σ'.exprs.toList = true := by grind
+        have : σ.exprs.toList <+: σ'.exprs.toList := by grind
+        have := List.prefix_iff_getElem?.mp this cache.size (by grind)
+        grind
+      rewrite [this]
+      split
+      . rfl
+      . simp
+        apply ih
+        grind
+
+
+
+end Prefix
 
 end Clap.HashConsM
